chore(examples): Improve insertion sort

examples/InsertionSort.v
@@ -15,137 +15,116 @@
    reasoning, uninterpreted functions, and a bit of integer arithmetic.
 
    Ideally, the proof of each lemma should consists only on
-   induction/destruct followed by a call to [smt]. What we currently
-   lack:
-     - we have to provide all the needed lemmas and unfold all the
-       definitions
-     - it requires too much from uninterpreted functions even when it is
-       not needed
-     - it sometimes fails (may be realted to the previous item)
+   induction/destruct followed by a call to [smt].
+
+   What we currently lack:
+    - we have to provide all the needed lemmas and unfold all the definitions
+    - it requires too much from uninterpreted functions even when it is not needed
+    - it sometimes fails (may be realted to the previous item)
  *)
 
 
-Require Import SMTCoq.SMTCoq.
-Require Import ZArith List Bool.
+From SMTCoq Require Import SMTCoq.
+From Stdlib Require Import Bool List ZArith.
 
 Local Open Scope Z_scope.
 
 
-(* This will improve when SMTCoq works with SSReflect! *)
+Fixpoint insert (x: Z) (l: list Z) : list Z :=
+  match l with
+  | nil => x :: nil
+  | y :: ys => if x <=? y then x :: y :: ys else y :: insert x ys
+  end.
 
-Lemma impl_implb (a b:bool) : (a -> b) <-> (a ---> b).
-Proof. auto using (reflect_iff _ _ (ReflectFacts.implyP a b)). Qed.
+Fixpoint sort (l: list Z) : list Z :=
+  match l with
+  | nil => nil
+  | x :: xs => insert x (sort xs)
+  end.
 
 
-Lemma eq_false b : b = false <-> negb b.
-Proof. case b; intuition. Qed.
+Section Spec.
+
+  (* This will improve when SMTCoq works with SSReflect! *)
+
+  Lemma impl_implb (a b: bool) : (a -> b) <-> (a ---> b).
+  Proof. apply reflect_iff, ReflectFacts.implyP. Qed.
+
+  Lemma eq_false b : b = false <-> negb b.
+  Proof. case b; intuition. Qed.
 
 
-Section InsertionSort.
-
-  Fixpoint insert (x:Z) (l:list Z) : list Z :=
+  Fixpoint is_sorted (l: list Z) : bool :=
     match l with
-    | nil => x::nil
-    | y::ys => if (x <=? y)%Z then x::y::ys else y::(insert x ys)
+    | nil => true
+    | x :: xs =>
+      match xs with
+      | nil => true
+      | y :: _ => (x <=? y) && is_sorted xs
+      end
     end.
 
-  Fixpoint sort (l:list Z) : list Z :=
+  Fixpoint smaller (x: Z) (l: list Z) : bool :=
     match l with
-    | nil => nil
-    | x::xs => insert x (sort xs)
+    | nil => true
+    | y :: ys => (x <=? y) && smaller x ys
     end.
 
+  Lemma is_sorted_smaller x y ys :
+    (x <=? y) && is_sorted (y :: ys) ---> is_sorted (x :: ys).
+  Proof.
+    destruct ys as [ | z zs]; simpl.
+    { now apply impl_implb. }
 
-  Section Spec.
+    smt.
+  Qed.
 
-    Fixpoint is_sorted (l:list Z) : bool :=
-      match l with
-      | nil => true
-      | x::xs =>
-        match xs with
-        | nil => true
-        | y::_ => (x <=? y)%Z && (is_sorted xs)
-        end
-      end.
+  Lemma is_sorted_cons x xs :
+    (is_sorted (x::xs)) <---> (is_sorted xs && smaller x xs).
+  Proof.
+    induction xs as [ | y ys IHys].
+    { reflexivity. }
 
-    Fixpoint smaller (x:Z) (l:list Z) : bool :=
-      match l with
-      | nil => true
-      | y::ys => (x <=? y)%Z && (smaller x ys)
-      end.
+    change (is_sorted (x :: y :: ys)) with ((x <=? y) && (is_sorted (y::ys))).
+    change (smaller x (y :: ys)) with ((x <=? y) && (smaller x ys)).
+    generalize (is_sorted_smaller x y ys).
+    smt.
+  Qed.
 
+  Lemma insert_keeps_smaller x y ys :
+    smaller y ys ---> (y <=? x) ---> smaller y (insert x ys).
+  Proof.
+    induction ys as [ | z zs IHzs]; simpl.
+    { smt. }
 
-    Lemma is_sorted_smaller x y ys :
-      (((x <=? y)%Z && is_sorted (y :: ys)) ---> is_sorted (x :: ys)).
-    Proof.
-      destruct ys as [ |z zs].
-      - simpl. smt.
-      - change (is_sorted (y :: z :: zs)) with ((y <=? z)%Z && (is_sorted (z::zs))).
-        change (is_sorted (x :: z :: zs)) with ((x <=? z)%Z && (is_sorted (z::zs))).
-        (* [smt] or [verit] fail? *)
-        assert (H:forall b, (x <=? y)%Z && ((y <=? z) && b) ---> (x <=? z) && b) by smt.
-        apply H.
-    Qed.
+    case (x <=? z); simpl.
+    - smt.
+    - smt.
+  Qed.
 
+  Lemma insert_keeps_sorted x l :
+    is_sorted l -> is_sorted (insert x l).
+  Proof.
+    induction l as [ | y ys IHys].
+    { reflexivity. }
 
-    Lemma is_sorted_cons x xs :
-      (is_sorted (x::xs)) <---> (is_sorted xs && smaller x xs).
-    Proof.
-      induction xs as [ |y ys IHys].
-      - reflexivity.
-      - change (is_sorted (x :: y :: ys)) with ((x <=? y)%Z && (is_sorted (y::ys))).
-        change (smaller x (y :: ys)) with ((x <=? y)%Z && (smaller x ys)).
-        generalize (is_sorted_smaller x y ys). revert IHys. rewrite !impl_implb.
-        (* Idem *)
-        assert (H:forall a b c d, (a <---> b && c) --->
-                                  ((x <=? y) && d ---> a) --->
-                                  ((x <=? y) && d <--->
-                                  d && ((x <=? y) && c))) by smt.
-        apply H.
-    Qed.
+    intro H; simpl.
+    case_eq (x <=? y); intro Heq.
+    - change ((x <=? y) && is_sorted (y :: ys)).
+      smt.
+    - rewrite eq_false in Heq.
+      rewrite (eqb_prop _ _ (is_sorted_cons _ _)) in H.
+      rewrite (eqb_prop _ _ (is_sorted_cons _ _)).
+      generalize (insert_keeps_smaller x y ys).
+      smt.
+  Qed.
 
+  Theorem sort_sorts l : is_sorted (sort l).
+  Proof.
+    induction l as [ | x xs IHxs].
+    { reflexivity. }
 
-    Lemma insert_keeps_smaller x y ys :
-      smaller y ys ---> (y <=? x) ---> smaller y (insert x ys).
-    Proof.
-      induction ys as [ |z zs IHzs].
-      - simpl. smt.
-      - simpl. case (x <=? z).
-        + simpl.
-          (* [smt] or [verit] require [Compec (list Z)] but they should not *)
-          assert (H:forall a, (y <=? z) && a ---> (y <=? x) ---> (y <=? x) && ((y <=? z) && a)) by smt.
-          apply H.
-        + simpl. revert IHzs. rewrite impl_implb.
-          (* Idem *)
-          assert (H:forall a b, (a ---> (y <=? x) ---> b) ---> (y <=? z) && a ---> (y <=? x) ---> (y <=? z) && b) by smt.
-          apply H.
-    Qed.
+    now apply insert_keeps_sorted.
+  Qed.
 
-
-    Lemma insert_keeps_sorted x l : is_sorted l -> is_sorted (insert x l).
-    Proof.
-      induction l as [ |y ys IHys].
-      - reflexivity.
-      - intro H. simpl. case_eq (x <=? y); intro Heq.
-        + change ((x <=? y)%Z && (is_sorted (y::ys))). rewrite Heq, H. reflexivity.
-        + rewrite eq_false in Heq.
-          rewrite (eqb_prop _ _ (is_sorted_cons _ _)) in H.
-          rewrite (eqb_prop _ _ (is_sorted_cons _ _)).
-          generalize (insert_keeps_smaller x y ys).
-          revert IHys H Heq. rewrite !impl_implb.
-          (* Idem *)
-          assert (H: forall a b c d, (a ---> b) ---> a && c ---> negb (x <=? y) ---> (c ---> (y <=? x) ---> d) ---> b && d) by smt.
-          apply H.
-    Qed.
-
-
-    Theorem sort_sorts l : is_sorted (sort l).
-    Proof.
-      induction l as [ |x xs IHxs].
-      - reflexivity.
-      - simpl. now apply insert_keeps_sorted.
-    Qed.
-
-  End Spec.
-
-End InsertionSort.
+End Spec.
